txn-data-consistency/EP+_TCCv_proof.thy
@@ -1989,6 +1989,67 @@ next
   qed (auto simp add: Kvt_map_t_Committed_def tps_trans_defs)
 qed
 
+subsection \<open>Kvt_map values meaning for read_done\<close>
+definition Rtxn_IdleK_notin_rs where
+  "Rtxn_IdleK_notin_rs s cl \<longleftrightarrow> (\<forall>k keys kvt_map t cts v rs deps.
+    cl_state (cls s cl) = RtxnInProg keys kvt_map \<and> k \<notin> keys \<and>
+    svr_state (svrs s k) t = Commit cts v rs deps \<longrightarrow> get_txn s cl \<notin> rs)"
+
+lemmas Rtxn_IdleK_notin_rsI = Rtxn_IdleK_notin_rs_def[THEN iffD2, rule_format]
+lemmas Rtxn_IdleK_notin_rsE[elim] = Rtxn_IdleK_notin_rs_def[THEN iffD1, elim_format, rule_format]
+
+lemma reach_rtxn_idle_k_notin_rs [simp]: "reach tps s \<Longrightarrow> Rtxn_IdleK_notin_rs s cl"
+proof(induction s rule: reach.induct)
+  case (reach_init s)
+  then show ?case by (auto simp add: Rtxn_IdleK_notin_rs_def tps_defs)
+next
+  case (reach_trans s e s')
+  then show ?case 
+  proof (induction e)
+    case (RInvoke x1 x2)
+    then show ?case apply (auto simp add: Rtxn_IdleK_notin_rs_def tps_trans_defs)
+      using Fresh_wr_notin_rs_def[of s]
+      by (metis dual_order.eq_iff insertCI reach_fresh_wr_notin_rs txid0.sel(1) txid0.sel(2))
+  next
+    case (RegR x1 x2 x3 x4)
+    then show ?case by (auto simp add: Rtxn_IdleK_notin_rs_def tps_trans_defs add_to_readerset_def
+          split: ver_state.split, blast+)
+  qed (auto simp add: Rtxn_IdleK_notin_rs_def tps_trans_defs, (blast+)?)
+qed
+
+definition Rtxn_RegK_in_rs where
+  "Rtxn_RegK_in_rs s cl \<longleftrightarrow> (\<forall>k keys kvt_map t cts v rs deps.
+    cl_state (cls s cl) = RtxnInProg keys kvt_map \<and> kvt_map k = Some (v, t) \<and>
+    svr_state (svrs s k) t = Commit cts v rs deps \<longrightarrow> get_txn s cl \<in> rs)"
+
+lemmas Rtxn_RegK_in_rsI = Rtxn_RegK_in_rs_def[THEN iffD2, rule_format]
+lemmas Rtxn_RegK_in_rsE[elim] = Rtxn_RegK_in_rs_def[THEN iffD1, elim_format, rule_format]
+
+lemma reach_rtxn_reg_k_in_rs [simp]: "reach tps s \<Longrightarrow> Rtxn_RegK_in_rs s cl"
+proof(induction s rule: reach.induct)
+  case (reach_init s)
+  then show ?case by (auto simp add: Rtxn_RegK_in_rs_def tps_defs)
+next
+  case (reach_trans s e s')
+  then show ?case 
+  proof (induction e)
+    case (Read x1 x2 x3 x4)
+    then show ?case apply (auto simp add: Rtxn_RegK_in_rs_def tps_trans_defs)
+      by (metis old.prod.inject option.inject ver_state.inject(2))
+  next
+    case (RegR x1 x2 x3 x4)
+    then show ?case by (auto simp add: Rtxn_RegK_in_rs_def tps_trans_defs add_to_readerset_def
+          split: ver_state.split; blast)
+  next
+    case (PrepW x1 x2 x3)
+    then show ?case by (simp add: Rtxn_RegK_in_rs_def tps_trans_defs, blast)
+  next
+    case (CommitW x1 x2 x3 x4 x5)
+    then show ?case apply (simp add: Rtxn_RegK_in_rs_def tps_trans_defs)
+      by (metis Kvt_map_t_Committed_def is_prepared.simps(3) reach_kvt_map_t_committed)
+  qed (auto simp add: Rtxn_RegK_in_rs_def tps_trans_defs)
+qed
+
 
 subsection \<open>Timestamp relations\<close>
 
@@ -2210,6 +2271,8 @@ lemma insert_kt_to_deps_closed':
 
 
 \<comment> \<open>concrete read_done closedness\<close>
+
+\<comment> \<open>premises\<close>
 lemma get_ctx_reformulate:
   assumes "cl_state (cls s cl) = RtxnInProg keys kvt_map"
     and "Kvt_map_t_Committed s cl"
@@ -2229,6 +2292,81 @@ lemma get_ctx_closed:
   shows "closed' K (get_ctx s kvt_map) r"
   using assms
   by (auto simp add: get_ctx_reformulate Finite_Dom_Kvt_map_def Let_def intro!: Union_closed')
+
+lemma v_writer_kvs_of_s:
+  assumes "\<forall>k. Commit_Order_Sound' s k"
+  shows "v_writer ` (\<lambda>t. case svr_state (svrs s k) t of
+      Prep ts v \<Rightarrow> \<lparr>v_value = v, v_writer = t, v_readerset = {}\<rparr>
+    | Commit cts v rs deps \<Rightarrow> \<lparr>v_value = v, v_writer = t,
+        v_readerset = {t \<in> rs. get_sn t < cl_sn (cls s (get_cl t))}\<rparr>) ` set (commit_order s k) =
+   {t \<in> set (commit_order s k). \<exists>ts v cts rs deps. svr_state (svrs s k) t \<in> {Prep ts v, Commit cts v rs deps}}"
+  using assms
+  by (auto simp add: image_iff Commit_Order_Sound'_def split: ver_state.split)
+
+lemma v_readerset_kvs_of_s_k:
+  assumes "\<forall>k. Commit_Order_Sound' s k"
+    and "t_wr \<in> set (commit_order s k)"
+  shows "v_readerset (case svr_state (svrs s k) t_wr of
+      Prep ts v \<Rightarrow> \<lparr>v_value = v, v_writer = t_wr, v_readerset = {}\<rparr>
+    | Commit cts v rs deps \<Rightarrow> \<lparr>v_value = v, v_writer = t_wr,
+        v_readerset = {t \<in> rs. get_sn t < cl_sn (cls s (get_cl t))}\<rparr>) = 
+   {t. \<exists>cts v rs deps. svr_state (svrs s k) t_wr = Commit cts v rs deps \<and>
+      t \<in> rs \<and> get_sn t < cl_sn (cls s (get_cl t))}"
+  using assms
+  by (auto split: ver_state.split)
+
+lemma v_readerset_kvs_of_s:
+  assumes "\<forall>k. Commit_Order_Sound' s k"
+  shows "(\<Union>k. \<Union>t_wr\<in>set (commit_order s k). v_readerset (case svr_state (svrs s k) t_wr of
+      Prep ts v \<Rightarrow> \<lparr>v_value = v, v_writer = t_wr, v_readerset = {}\<rparr>
+    | Commit cts v rs deps \<Rightarrow> \<lparr>v_value = v, v_writer = t_wr,
+        v_readerset = {t \<in> rs. get_sn t < cl_sn (cls s (get_cl t))}\<rparr>)) = 
+   {t. \<exists>k. \<exists>t_wr \<in> set (commit_order s k).
+      \<exists>cts v rs deps. svr_state (svrs s k) t_wr = Commit cts v rs deps \<and>
+      t \<in> rs \<and> get_sn t < cl_sn (cls s (get_cl t))}"
+  using assms
+  apply (auto simp add: v_readerset_kvs_of_s_k)
+  by blast+
+
+lemma read_done_same_writers:
+  assumes "read_done cl kvt_map sn u'' s s'"
+    and "\<forall>k. Commit_Order_Sound' s k"
+    and "\<forall>k. Commit_Order_Sound' s' k"
+  shows "kvs_writers (kvs_of_s s') = kvs_writers (kvs_of_s s)"
+  using assms
+  apply (simp add: kvs_writers_def vl_writers_def kvs_of_s_def v_writer_kvs_of_s Commit_Order_Sound'_def)
+  by (simp add: read_done_def)
+
+lemma insert_Diff_if': "a \<notin> c \<Longrightarrow> insert a (b - c) = insert a b - c"
+  by (simp add: insert_Diff_if)
+
+lemma read_done_new_read:
+  assumes "read_done cl kvt_map sn u'' s s'"
+    and "\<forall>k. Commit_Order_Sound' s k"
+    and "\<forall>k. Commit_Order_Sound' s' k"
+    and "\<forall>k. Commit_Order_Complete s k"
+    and "\<forall>k. Commit_Order_T0 s k"
+    and "Finite_Dom_Kvt_map s cl"
+    and "Kvt_map_t_Committed s cl"
+    and "Rtxn_RegK_in_rs s cl"
+    and "Tn (get_txn s cl) \<notin> kvs_writers (kvs_of_s s)"
+  shows "read_only_Txs (kvs_of_s s') = insert (Tn (get_txn s cl)) (read_only_Txs (kvs_of_s s))"
+  using assms
+  apply (simp add: read_only_Txs_def read_done_same_writers insert_Diff_if')
+  apply (rule arg_cong[where f="\<lambda>m. m - _"])
+  apply (simp add: kvs_readers_def vl_readers_def kvs_of_s_def v_readerset_kvs_of_s)
+  apply (auto simp add: read_done_def image_insert[symmetric] simp del: image_insert)
+  using image_eqI apply blast
+  apply (smt (z3) image_eqI insertCI less_SucE mem_Collect_eq txid0.collapse)
+  using image_eqI apply blast
+  subgoal apply (rule image_eqI, auto)
+    apply (cases "dom kvt_map = {}", auto simp add: ex_in_conv[symmetric] simp del: dom_eq_empty_conv)
+    subgoal for k v t apply (rule exI[where x=k]) apply (rule bexI[where x=t])
+      apply (smt (verit) Kvt_map_t_Committed_def Rtxn_RegK_in_rs_def)
+      apply (cases t, blast)
+      by (metis (no_types, lifting) Kvt_map_t_Committed_def Commit_Order_Complete_def txid0.exhaust)
+    done
+  by (smt (verit) image_eqI less_Suc_eq mem_Collect_eq)
 
 lemma fresh_rtxn_not_vis:
   assumes "Tn (get_txn s cl) \<notin> kvs_writers (kvs_of_s s)"
@@ -2250,6 +2388,7 @@ lemma read_done_extend_rel:
   using assms
   by (auto simp add: R_CC_def read_done_WR_onK)
 
+\<comment> \<open>read_done closedness (canCommit)\<close>
 lemma read_done_ctx_closed:
   assumes "closed' (kvs_of_s s) (cl_ctx (cls s cl)) (R_CC (kvs_of_s s))"
     and "closed' (kvs_of_s s) (get_ctx s kvt_map) (R_CC (kvs_of_s s))"
